specIR/SIREuttLocal.v
@@ -1,0 +1,116 @@
+From Coq Require Import
+     Arith.PeanoNat
+     Lists.List
+     Strings.String
+     Morphisms
+     Setoid
+     RelationClasses.
+
+Require Import MapsC.
+Require Import ValuesC.
+Require Import MemoryC.
+Require Import CoqlibC.
+Require Import ASTC.
+Require Import EventsC.
+Require Import GlobalenvsC.
+Require Import IntegersC.
+Require Import Mod ModSem Any Skeleton.
+Require Import SimMem SimSymb Sound.
+Require SimMemId SimSymbId SoundTop.
+Require Import SimMod SimModSem.
+Require Import SIRCommon SIR SimSIR.
+
+Require Import Program.
+Require Import Simulation.
+Require Import SIREuttGlobal.
+
+Set Implicit Arguments.
+
+Local Open Scope signature_scope.
+
+
+
+
+Section OWNEDHEAP.
+
+Variable mi: string.
+Variable owned_heap: Type.
+
+
+
+
+
+(*** sim syntax ***)
+Section SYNTAX.
+
+(*** sim itree ***)
+Let itr := itree (E owned_heap) (owned_heap * (mem * val)).
+
+Definition match_itr: relation itr := fun i_src i_tgt => i_src ≈ i_tgt.
+
+Let fn := function owned_heap.
+
+Definition match_fn: relation (function owned_heap) := (eq ==> eq ==> eq ==> match_itr).
+
+Definition match_prog: relation (program owned_heap) := (eq ==> option_rel match_fn).
+
+End SYNTAX.
+Hint Unfold match_itr match_fn match_prog.
+
+Lemma match_prog_local_global_aux
+      p_src p_tgt
+      (SIMP: match_prog p_src p_tgt)
+  :
+    Relation.i_pointwise (fun _ => eutt eq) (interp_function p_src) (interp_function p_tgt)
+.
+Proof.
+  ii.
+  destruct a; ss.
+  r in SIMP. exploit (SIMP name); et. intro U. rr in U. des_ifs; et.
+  - eapply U; et.
+  - refl.
+Qed.
+
+Theorem match_prog_local_global
+        (p_src p_tgt: program owned_heap)
+        (SIMP: match_prog p_src p_tgt)
+  :
+    (<<SIMP: SIREuttGlobal.match_prog p_src p_tgt>>)
+.
+Proof.
+  ii.
+  eapply Proper_interp_mrec; et.
+  - eapply match_prog_local_global_aux; et.
+  - eapply match_prog_local_global_aux; et.
+Qed.
+
+
+
+
+
+Section SIM.
+
+  Variable md_src: SMod.t owned_heap.
+  Variable md_tgt: SMod.t owned_heap.
+  Let p_src := md_src.(SMod.prog).
+  Let p_tgt := md_tgt.(SMod.prog).
+  Let mi_src := md_src.(SMod.midx).
+  Let mi_tgt := md_tgt.(SMod.midx).
+  Hypothesis (SIMP: match_prog p_src p_tgt).
+  Hypothesis (SIMMI: mi_src = mi_tgt).
+  Hypothesis (SIMO: forall skenv, (md_src.(SMod.initial_owned_heap) skenv)
+                                  = (md_tgt.(SMod.initial_owned_heap) skenv)).
+  Hypothesis (SIMSK: md_src.(SMod.sk) = md_tgt.(SMod.sk)).
+  Let mp: ModPair.t := (SimSymbId.mk_mp md_src md_tgt).
+  Let SIMPG: SIREuttGlobal.match_prog p_src p_tgt. eapply match_prog_local_global; et. Qed.
+
+  Theorem sim_mod: ModPair.sim mp.
+  Proof. eapply SIREuttGlobal.sim_mod; et. Qed.
+
+  Theorem correct: rusc defaultR [md_src: Mod.t] [md_tgt: Mod.t].
+  Proof. eapply SIREuttGlobal.correct; et. Qed.
+
+End SIM.
+
+End OWNEDHEAP.
+Hint Unfold match_itr match_fn match_prog.
