specIR/SIRProps.v
@@ -2,4 +2,5 @@ Require Export SIRStackproof.
 Require Export SIRHoare.
 Require Export SimSIR.
 Require Export SIRLocal.
-Require Export SIREutt.
+Require Export SIREuttLocal.
+Require Export SIREuttGlobal.
